\documentclass[../notes.tex]{subfiles}

\pagestyle{main}
\renewcommand{\chaptermark}[1]{\markboth{\chaptername\ \thechapter\ (#1)}{}}
\setcounter{chapter}{3}

\begin{document}




\chapter{Observables and Hermitian Operators}
\section{Harmonic Oscillator: Raising and Lowering Operators}
\begin{itemize}
    \item \marginnote{1/22:}\textbf{Raising operator}: The operator defined as follows. \emph{Denoted by} $\bm{\hat{a}_+}$, $\bm{a_+}$. \emph{Given by}
    \begin{equation*}
        \hat{a}_+ = \frac{1}{\sqrt{2\hbar m\omega}}[-i\hat{\vec{p}}+m\omega\hat{\vec{x}}\,]
    \end{equation*}
    \item \textbf{Lowering operator}: The operator defined as follows. \emph{Denoted by} $\bm{\hat{a}_-}$, $\bm{a_-}$. \emph{Given by}
    \begin{equation*}
        \hat{a}_- = \frac{1}{\sqrt{2\hbar m\omega}}[i\hat{\vec{p}}+m\omega\hat{\vec{x}}\,]
    \end{equation*}
    \item \textbf{Number operator}: The operator defined as follows. \emph{Denoted by} $\bm{a_+a_-}$. \emph{Given by}
    \begin{equation*}
        a_+a_- = \hat{a}_+\circ\hat{a}_-
        = \frac{1}{2\hbar m\omega}\left[ \hat{\vec{p}}{\,}^2+m^2\omega^2x^2-im\omega[\hat{\vec{p}},\hat{\vec{x}}] \right]
    \end{equation*}
    \item Properties of these operators.
    \begin{itemize}
        \item We can express $\hat{\vec{p}},\hat{\vec{x}}$ in terms of $a_+,a_-$ via
        \begin{align*}
            \hat{\vec{p}} &= i\sqrt{\frac{\hbar m\omega}{2}}(\hat{a}_+-\hat{a}_-)&
            \hat{\vec{x}} &= \sqrt{\frac{\hbar}{2m\omega}}(\hat{a}_++\hat{a}_-)
        \end{align*}
        \begin{itemize}
            \item It follows that
            \begin{equation*}
                [\hat{\vec{p}},\hat{\vec{x}}] = \frac{i\hbar}{2}[a_+-a_-,a_++a_-]
                = \frac{i\hbar}{2}([a_+,a_-]-[a_-,a_+])
                = i\hbar[a_+,a_-]
            \end{equation*}
            \item Consequently, since $[\hat{\vec{p}},\hat{\vec{x}}]=-i\hbar$, we have that
            \begin{equation*}
                [a_+,a_-] = -1
            \end{equation*}
            \item We also have that
            \begin{equation*}
                [a_-,a_+] = 1
            \end{equation*}
        \end{itemize}
        \item Since $[\hat{\vec{p}},\hat{x}]=-i\hbar$ and $\omega^2=k/m$, we have that
        \begin{align*}
            a_+a_- &= \frac{1}{2\hbar m\omega}\left[ \hat{\vec{p}}{\,}^2+m^2\omega^2x^2-m\hbar\omega \right]\\
            &= \frac{1}{\hbar\omega}\Bigg[ \underbrace{\frac{\hat{\vec{p}}{\,}^2}{2m}+\frac{kx^2}{2}}_{\hat{H}}-\frac{\hbar\omega}{2} \Bigg]\\
            \hat{H} &= \hbar\omega\left( a_+a_-+\frac{1}{2} \right)
        \end{align*}
        \begin{itemize}
            \item Because of the properties of $[a_+,a_-]$ proven above, we similarly have that
            \begin{equation*}
                \hat{H} = \hbar\omega\left( a_-a_+-\frac{1}{2} \right)
            \end{equation*}
            \item We can also derive this equation in a manner exactly analogous to the first one.
        \end{itemize}
    \end{itemize}
    \item How does the number operator act on the eigenstate $\ket{\psi_n}$ of the harmonic oscillator?
    \begin{itemize}
        \item Since $E_n=\hbar\omega(n+1/2)$, we have that
        \begin{align*}
            \hbar\omega\left( a_+a_-+\frac{1}{2} \right)\ket{\psi_n} &= \hat{H}\ket{\psi_n}\\
            \hbar\omega\left( a_+a_-+\frac{1}{2} \right)\ket{\psi_n} &= \hbar\omega\left( n+\frac{1}{2} \right)\ket{\psi_n}\\
            a_+a_-\ket{\psi_n} &= n\ket{\psi_n}
        \end{align*}
    \end{itemize}
    \item How do the raising and lowering operators act on the eigenstate $\ket{\psi_n}$ of the harmonic oscillator?
    \begin{itemize}
        \item Using a number of the above substitutions, we have that
        \begin{align*}
            \hat{H}(a_+\ket{\psi_n}) &= \left[ \hbar\omega\left( a_+a_-+\frac{1}{2} \right) \right](a_+\ket{\psi_n})\\
            &= \hbar\omega\left( a_+a_-a_++\frac{1}{2}a_+ \right)\ket{\psi_n}\\
            &= \hbar\omega a_+\left( a_-a_++\frac{1}{2} \right)\ket{\psi_n}\\
            &= \hbar\omega a_+\left( a_+a_-+1+\frac{1}{2} \right)\ket{\psi_n}\\
            &= \hbar\omega a_+\left( n+1+\frac{1}{2} \right)\ket{\psi_n}\\
            &= E_{n+1}(a_+\ket{\psi_n})
        \end{align*}
        \item This means that $\hat{H}$ acts on $a_+\ket{\psi_n}$ the same way it acts on $\ket{\psi_{n+1}}$. In other words, it must be that
        \begin{equation*}
            a_+\ket{\psi_n} \propto \ket{\psi_{n+1}}
        \end{equation*}
        \item Similarly,
        \begin{equation*}
            \hat{H}(a_-\ket{\psi_n}) = E_{n-1}(a_-\ket{\psi_n})
        \end{equation*}
        so
        \begin{equation*}
            a_-\ket{\psi_n} \propto \ket{\psi_{n-1}}
        \end{equation*}
        \item These actions are why $a_+,a_-$ are called the \emph{raising} and \emph{lowering} operators!
        \item We now seek to determine the constants of proportionality.
        \item First off, note that $a_+$ and $a_-$ are adjoints, i.e.,
        \begin{equation*}
            a_+^\dagger = a_-
        \end{equation*}
        \begin{itemize}
            \item This identity is evident from the original $\hat{a}_+,\hat{a}_-$ definitions, where the only difference between the two definitions is the conjugacy of the imaginary momentum term!
            \item Is this correct, or do I have to appeal to the formal $\braket{\psi_i}{\hat{a}_+\psi_j}=\braket*{\hat{a}_+^\dagger\psi_i}{\psi_j}$ definition??
        \end{itemize}
        \item Then for $a_+$, we know that if
        \begin{align*}
            a_+\ket{\psi_n} = c_+\ket{\psi_n}
        \end{align*}
        then
        \begin{align*}
            c_+^2 &= c_+^2\braket{\psi_{n+1}}\\
            &= \braket{c_+\psi_{n+1}}\\
            &= \braket{a_+\psi_n}\\
            &= \ev{a_+^\dagger a_+}{\psi_n}\\
            &= \ev{a_-a_+}{\psi_n}\\
            &= \ev{a_+a_-+1}{\psi_n}\\
            &= (n+1)\braket{\psi_n}\\
            &= n+1
        \end{align*}
        so that, taking square roots,
        \begin{equation*}
            c_+ = \sqrt{n+1}
        \end{equation*}
        \item By the same method --- namely
        \begin{equation*}
            c_-^2 = \braket{a_-\psi_n}
            = \ev{a_+a_-}{\psi_n}
            = n
        \end{equation*}
        we can also learn that
        \begin{equation*}
            c_- = \sqrt{n}
        \end{equation*}
        \item Therefore,
        \begin{align*}
            a_+\ket{\psi_n} &= \sqrt{n+1}\ket{\psi_{n+1}}&
            a_-\ket{\psi_n} &= \sqrt{n}\ket{\psi_{n-1}}
        \end{align*}
        \item Note that what we have done here to derive this fact is far more slick than working directly with the unintuitive and complicated formal definitions of $a_+,a_-$.
    \end{itemize}
    \item Now is a good time to mention a bit more about Dirac notation.
    \begin{itemize}
        \item A "ket" represents a vector in a Hilbert space, so $\ket{\psi_n}$ demonstrates that we are talking about the wave function as a vector in the abstract linear algebra sense, not as a function $\psi_n:\R^4\to\C$.
        \item A "bra" represents a linear functional on a Hilbert space. In quantum mechanics, the linear functional $\bra{\eta}$ is given by
        \begin{equation*}
            \bra{\eta} := \int\dd^3\vec{r}\ \eta^*
        \end{equation*}
        \item Observe that this "functional" does indeed map any $\ket{\psi_n}$ given to it as an argument to a number $\braket{\eta}{\psi_n}$!
    \end{itemize}
    \item $\ket{\psi_n}$ can be defined in terms of $a_+$, $\ket{\psi_0}$, and constants.
    \begin{itemize}
        \item Observe that since $a_+\ket{\psi_0}=\ket{\psi_1}$ and $a_+\ket{\psi_1}=\sqrt{2}\ket{\psi_2}$, we have that
        \begin{equation*}
            \ket{\psi_2} = \frac{a_+}{\sqrt{2}}\ket{\psi_1}
            = \frac{a_+^2}{\sqrt{2}}\ket{\psi_0}
        \end{equation*}
        \item Similarly,
        \begin{equation*}
            \ket{\psi_3} = \frac{a_+}{\sqrt{3}}\ket{\psi_2}
            = \frac{a_+^3}{\sqrt{3\cdot 2}}\ket{\psi_0}
        \end{equation*}
        \item Generalizing, we have that
        \begin{equation*}
            \ket{\psi_n} = \frac{a_+^n}{\sqrt{n!}}\ket{\psi_0}
        \end{equation*}
    \end{itemize}
    \item Thus, we have that
    \begin{equation*}
        \psi_n(x) = \left( \frac{1}{\sqrt{2\hbar m\omega}} \right)^n\frac{1}{\sqrt{n!}}\left( -\hbar\dv{x}+xm\omega \right)^n\psi_0(x)
    \end{equation*}
    where we may recall that
    \begin{equation*}
        \psi_0(x) = \left( \frac{m\omega}{\hbar\pi} \right)^{1/4}\e[-m\omega x^2/2\hbar]
    \end{equation*}
    \item Final observations about the raising and lowering operators.
    \begin{itemize}
        \item Since $a_-\ket{\psi_0}=0$ (as we may readily verify by direct computation), we have that
        \begin{equation*}
            \hbar\dv{\psi_0}{x}+m\omega x\psi_0 = 0
        \end{equation*}
        \item We also know that
        \begin{equation*}
            \dd(\ln(\psi_0)) = -\frac{m\omega}{\hbar}\frac{\dd{x}^2}{2}
        \end{equation*}
        so
        \begin{equation*}
            \psi_0 \propto \e[-m\omega x^2/2\hbar]
        \end{equation*}
        \begin{itemize}
            \item What is the point of this line?? What new information does it give us?
        \end{itemize}
    \end{itemize}
    \item Raising and lowering operators allow us to compute the kinetic and potential energy of the harmonic oscillator.
    \begin{itemize}
        \item Kinetic energy.
        \begin{align*}
            \ev**{\frac{\hat{\vec{p}}{\,}^2}{2m}}{\psi_n} &= -\frac{\hbar\omega}{4}\ev{(a_+-a_-)^2}{\psi_n}\\
            &= -\frac{\hbar\omega}{4}\ev{a_+^2+a_-^2-a_+a_--a_-a_+}{\psi_n}\\
            % &= -\frac{\hbar\omega}{4}\left[ \ev{a_+^2}{\psi_n}+\ev{a_-^2}{\psi_n}-2\ev{a_+a_-}{\psi_n}-\ev{1}{\psi_n} \right]\\
            &= -\frac{\hbar\omega}{4}\big[ \underbrace{\ev{a_+^2}{\psi_n}}_{\propto\,\braket{\psi_n}{\psi_{n+2}}}+\underbrace{\ev{a_-^2}{\psi_n}}_{\propto\,\braket{\psi_n}{\psi_{n-2}}}-\underbrace{2\ev{a_+a_-}{\psi_n}}_{2n\braket{\psi_n}}-\underbrace{\ev{1}{\psi_n}}_{\braket{\psi_n}} \big]\\
            &= \frac{\hbar\omega}{4}(2n+1)\\
            &= \frac{\hbar\omega}{2}\left( n+\frac{1}{2} \right)\\
            &= \frac{E_n}{2}
        \end{align*}
        \item Potential energy.
        \begin{align*}
            \ev{\hat{H}}{\psi_n} &= E_n\\
            \ev**{\frac{\hat{\vec{p}}{\,}^2}{2m}}{\psi_n}+\ev**{k\frac{\hat{\vec{x}}{\,}^2}{2}}{\psi_n} &= \frac{E_n}{2}+\frac{E_n}{2}\\
            \ev**{k\frac{\hat{\vec{x}}{\,}^2}{2}}{\psi_n} &= \frac{E_n}{2}
        \end{align*}
        \item Implication: In an energy eigenstate, the harmonic oscillator has equal values of kinetic and potential energies!
    \end{itemize}
    \pagebreak
    \item Computing more observables.
    \begin{itemize}
        \item We can show that
        \begin{align*}
            \ev{\hat{\vec{x}}}{\psi_n} &= \ev{\hat{\vec{p}}\,}{\psi_n} = 0&
            \ev{\hat{\vec{x}}{\,}^2}{\psi_n} &= \frac{\hbar\omega}{k}\left( n+\frac{1}{2} \right)&
            \ev{\hat{\vec{p}}{\,}^2}{\psi_n} &= \hbar\omega m\left( n+\frac{1}{2} \right)
        \end{align*}
    \end{itemize}
    \item It follows from the above computations and the facts that
    \begin{align*}
        \Delta x^2 &= \ev{\hat{\vec{x}}{\,}^2}{\psi_n}-(\ev{\hat{\vec{x}}}{\psi_n})^2&
        \Delta p^2 &= \ev{\hat{\vec{p}}{\,}^2}{\psi_n}-(\ev{\hat{\vec{p}}\,}{\psi_n})^2
    \end{align*}
    that
    \begin{align*}
        \Delta x^2\cdot\Delta p^2 &= \hbar^2\left( n+\frac{1}{2} \right)^2\\
        \Delta x\cdot\Delta p &= \frac{\hbar}{2}(2n+1)
    \end{align*}
    \begin{itemize}
        \item Implication: The ground state $\psi_0(x)$ is represented by a Gaussian since in this case, $\Delta x\cdot\Delta p=\hbar/2$.
    \end{itemize}
    \item Review from last class.
    \begin{itemize}
        \item Mostly stuff I already wrote down.
        \item One new equation formalizing the even/odd solutions:
        \begin{equation*}
            f_n(x) = (-1)^nf_n(-x)
        \end{equation*}
        \item The first four Hermite polynomials:
        \begin{align*}
            H_0(\xi) &= 1&
            H_1(\xi) &= 2\xi&
            H_2(\xi) &= 4\xi^2-2&
            H_3 &= 8\xi^3-12\xi
        \end{align*}
        \item Summary of the characteristics of $E_n$: The energy is quantized and grows linearly with $n$ in quanta of $\hbar\omega$, and has a minimum value $\hbar\omega/2$.
        \item As with other time-independent potentials, the general solution to the Schr\"{o}dinger equation will be
        \begin{equation*}
            \psi(x,t) = \sum_nc_n\psi_n(x)\e[-iE_nt/\hbar]
        \end{equation*}
        where
        \begin{equation*}
            \ev{\hat{H}}{\psi} = \sum_n|c_n|^2E_n
        \end{equation*}
    \end{itemize}
\end{itemize}



\section{Time Dependence and Coherent States}
\begin{itemize}
    \item \marginnote{1/24:}Review of the harmonic oscillator.
    \begin{itemize}
        \item Our Hamiltonian is
        \begin{equation*}
            \hat{H} = -\frac{\hbar^2}{2m}\dv[2]{x}+\frac{kx^2}{2} = \frac{\hat{\vec{p}}{\,}^2}{2m}+\frac{k\hat{\vec{x}}{\,}^2}{2}
        \end{equation*}
        \begin{itemize}
            \item We have an analogy with the classical $\omega^2=k/m$.
        \end{itemize}
        \item Under this Hamiltonian, $\hat{H}\ket{\psi_n}=E_n\ket{\psi_n}$ implies that
        \begin{equation*}
            E_n = \hbar\omega\left( \frac{1}{2}+n \right)
        \end{equation*}
        \item The raising and lowering operators are given by
        \begin{align*}
            a_+ &= \frac{1}{\sqrt{2\hbar m\omega}}[-i\hat{\vec{p}}+m\omega\hat{\vec{x}}\,]&
            a_- &= \frac{1}{\sqrt{2\hbar m\omega}}[i\hat{\vec{p}}+m\omega\hat{\vec{x}}\,]
        \end{align*}
        \begin{itemize}
            \item Together, these imply that
            \begin{equation*}
                \hat{H} = \hbar\omega\left( a_+a_-+\frac{1}{2} \right)
            \end{equation*}
            \item We also have that
            \begin{align*}
                a_+a_-\ket{\psi_n} &= n\ket{\psi_n}&
                    a_+\ket{\psi_n} &= \sqrt{n+1}\ket{\psi_{n+1}}\\
                [a_-,a_+] &= 1&
                    a_-\ket{\psi_n} &= \sqrt{n}\ket{\psi_{n-1}}
            \end{align*}
            \item We call $a_+a_-$ the number operator.
            \item We should go home and learn these formulas.
        \end{itemize}
        \item The full eigenstate is
        \begin{equation*}
            \psi(x,t) = \sum_{n=0}^\infty\underbrace{c_n\psi_n(x)\e[-iE_nt/\hbar]}_{\psi_n(x,t)}
        \end{equation*}
        \item Two properties of this eigenstate.
        \begin{enumerate}
            \item We have that
            \begin{equation*}
                \ket{\psi} = \sum_{n=0}^\infty c_n\e[-iE_nt/\hbar]\ket{\psi_n}
            \end{equation*}
            which implies that
            \begin{equation*}
                \sum_{n=0}^\infty|c_n|^2 = 1
            \end{equation*}
            since $\braket{\psi}=1$ and $\braket{\psi_n}{\psi_m}=\delta_{nm}$.
            \item We have that
            \begin{equation*}
                \ev{\hat{H}}{\psi} = \sum_{n=0}^\infty|c_n|^2E_n
            \end{equation*}
        \end{enumerate}
        \item We have that
        \begin{align*}
            \ev**{\frac{k\hat{\vec{x}}{\,}^2}{2}}{\psi_n} &= \frac{\hbar\omega}{2}\left( n+\frac{1}{2} \right) = \frac{E_n}{2}&
            \ev**{\frac{\hat{\vec{p}}{\,}^2}{2m}}{\psi_n} &= \frac{\hbar\omega}{2}\left( n+\frac{1}{2} \right) = \frac{E_n}{2}
        \end{align*}
        \begin{itemize}
            \item Note that this makes sense because the sum $E_n/2+E_n/2$ of potential and kinetic should be $E_n$, and it will be!
        \end{itemize}
        \item Additionally, recall that we have
        \begin{align*}
            \hat{\vec{p}}{\,}^2 &\propto (a_+-a_-)^2&
            \hat{\vec{x}}{\,}^2 &\propto (a_++a_-)^2
        \end{align*}
        \begin{itemize}
            \item Thus, we have that
            \begin{align*}
                \ev{\hat{\vec{p}}\,}{\psi_n} &= \ev{(a_+-a_-)}{\psi_n} = 0&
                \ev{\hat{\vec{x}}}{\psi_n} &= \ev{(a_++a_-)}{\psi_n} = 0
            \end{align*}
        \end{itemize}
        \item The harmonic oscillator is a very important problem in physics, and we should know it by heart! (In order to pass the class.)
    \end{itemize}
    \item Recall as well that there is a correspondence between the Dirac notation and the functional notation, given by
    \begin{equation*}
        \psi_n(x) \mapsto \ket{\psi_n}
    \end{equation*}
    \begin{itemize}
        \item As an additional example,
        \begin{equation*}
            \frac{1}{\sqrt{2\hbar m\omega}}\left[ -\hbar\dv{x}+m\omega x \right]\psi_n(x) = \sqrt{n+1}\psi_{n+1}(x)
            \quad\mapsto\quad
            a_+\ket{\psi_n} = \sqrt{n+1}\ket{\psi_{n+1}}
        \end{equation*}
        \item One more example:
        \begin{equation*}
            \hbar\dv{\psi_0}{x}+m\omega x\psi_0(x) = 0
            \quad\mapsto\quad
            a_-\ket{\psi_0} = 0
        \end{equation*}
        \begin{itemize}
            \item Note that solving this ODE yields the solution
            \begin{equation*}
                \psi_0 = C\exp(-\frac{m\omega x^2}{2\hbar})
            \end{equation*}
            \item It appears that this is how we intuitively derive the ansatz we used last Friday!
        \end{itemize}
    \end{itemize}
    \item Now we start on some new content.
    \item Observe that
    \begin{align*}
        \frac{2m\omega\hat{\vec{x}}}{\sqrt{2\hbar m\omega}} &= a_++a_-\\
        \hat{\vec{x}} &= \sqrt{\frac{\hbar}{2m\omega}}(a_++a_-)
    \end{align*}
    \item In classical mechanics, the solution to the harmonic oscillator is
    \begin{equation*}
        x(t) = A\sin\omega t+B\cos\omega t
    \end{equation*}
    \item We now investigate the observables of $\ket{\psi}$.
    \item To start with, we show how $\ev{\hat{\vec{x}}}{\psi}$ varies with time. This will lead into a discussion of something called coherent states. Let's begin.
    \begin{itemize}
        \item We start with
        \begin{equation*}
            \ev{\hat{\vec{x}}}{\psi} = \sum_{m,n=0}^\infty c_m^*c_n\e[i(E_m-E_n)t/\hbar]\mel{\psi_n}{\hat{\vec{x}}}{\psi_n}
        \end{equation*}
        \item We can algebraically manipulate the above to
        \begin{align*}
            \ev{\hat{\vec{x}}}{\psi} ={}& \sum_{m,n=0}^\infty c_m^*c_n\e[i(\hbar\omega(m-n))t/\hbar]\sqrt{\frac{\hbar}{2m\omega}}\left( \sqrt{n+1}\delta_{m,n+1}+\sqrt{n}\delta_{m,n-1} \right)\\
            ={}& \sum_{n=0}^\infty c_{n+1}^*c_n\e[i\omega t]\sqrt{\frac{\hbar}{2m\omega}}\sqrt{n+1}+\sum_{n=1}^\infty c_{n-1}^*c_n\e[-i\omega t]\sqrt{\frac{\hbar}{2m\omega}}\sqrt{n}\\
            ={}& \sum_{n=0}^\infty c_{n+1}^*c_n\e[i\omega t]\sqrt{\frac{\hbar}{2m\omega}}\sqrt{n+1}+\sum_{n=0}^\infty c_n^*c_{n+1}\e[-i\omega t]\sqrt{\frac{\hbar}{2m\omega}}\sqrt{n+1}\\
            \begin{split}
                ={}& \sqrt{\frac{\hbar}{2m\omega}}\cos(\omega t)\left[ \sum_{n=0}^\infty\left( c_{n+1}^*c_n+c_n^*c_{n+1} \right)\sqrt{n+1} \right]\\
                & +\sqrt{\frac{\hbar}{2m\omega}}\sin(\omega t)\left[ \sum_{n=0}^\infty\left( c_{n+1}^*c_n-c_n^*c_{n+1} \right)\sqrt{n+1} \right]
            \end{split}
        \end{align*}
        \item Thus,
        \begin{equation*}
            \ev{\hat{\vec{x}}}{\psi} = A\cos\omega t+B\sin\omega t
        \end{equation*}
        where
        \begin{align*}
            A &= 2\re\left[ \sum_{n=0}^\infty c_{n+1}^*c_n\sqrt{n+1} \right]\sqrt{\frac{\hbar}{2m\omega}}&
                B &= 2\im\left[ \sum_{n=0}^\infty c_{n+1}^*c_n\sqrt{n+1} \right]\sqrt{\frac{\hbar}{2m\omega}}\\
            &= \re\left[ \sum_{n=0}^\infty c_{n+1}^*c_n\sqrt{n+1} \right]\sqrt{\frac{2\hbar}{m\omega}}&
                &= \im\left[ \sum_{n=0}^\infty c_{n+1}^*c_n\sqrt{n+1} \right]\sqrt{\frac{2\hbar}{m\omega}}
        \end{align*}
        \item Now for large values of $n$,
        \begin{equation*}
            \sqrt{n+1}\sqrt{\frac{2\hbar}{m\omega}} = \sqrt{\frac{2\hbar\omega(n+1)}{m\omega^2}}
            \approx \sqrt{\frac{2E_n}{m\omega^2}}
        \end{equation*}
        where
        \begin{align*}
            E_n &= \hbar\omega\left( n+\frac{1}{2} \right)&
            x &= A\sin\omega t&
            E &= \frac{m\omega^2A^2}{2}&
            A &= \sqrt{\frac{2E}{m\omega^2}}
        \end{align*}
        \begin{itemize}
            \item How can we just ignore the real and imaginary sum terms??
        \end{itemize}
        \item Now take the harmonic oscillator. Notice that $\sum_n$ is dominated by large values of $n\approx\bar{n}$, close to $\bar{n}$, where $\bar{n}\gg 1$. Thus,
        \begin{equation*}
            \ev{\hat{\vec{x}}}{\psi} = \sqrt{\frac{2E\bar{n}}{m\omega^2}}\sum_{n=0}^\infty\re\left[ \sum c_{n+1}^*c_n \right]\sin\omega t
        \end{equation*}
        and
        \begin{equation*}
            \ev{\hat{\vec{x}}{\,}^2}{\psi}-(\ev{\hat{\vec{x}}}{\psi})^2 \neq 0
        \end{equation*}
        \item This is \emph{not} classical motion.
        \item The states that come closest to realizing classical motion are called \textbf{coherent states}.
    \end{itemize}
    \item \textbf{Coherent state}: A state in which the uncertainty in $\hat{\vec{x}}$ is minimized.
    \item Example:
    \begin{itemize}
        \item We have that
        \begin{align*}
            a_-\ket{\alpha} &= \alpha\ket{\alpha}&
            a_-\ket{\psi_0} &= 0\ket{\psi_0}
        \end{align*}
        \item Then
        \begin{align*}
            \frac{\hbar}{2m\omega}\left[ \ev{(a_++a_-)^2}{\alpha}-(\ev{(a_++a_-)}{\alpha})^2 \right] &= \frac{\hbar}{2}\\
            \frac{\hbar}{2m\omega}\left[ \ev{a_+^2+a_+a_-+a_-a_++a_-^2}{\alpha}-(\ev{(a_++a_-)}{\alpha})^2 \right] &= \dots
        \end{align*}
        \item We'll finish this up next time.
    \end{itemize}
\end{itemize}




\end{document}